---
title: "Untitled"
author: "a"
date: "26 September 2018"
output:
  pdf_document: default
  html_document: default
---

We use the derivative:


E=m*c^2

$\left( \begin{array}{r} y_1 \\ y_2 \\ y_3 \\ y_4 \\ y_5 \\ y_6 \\ y_7 \\ y_8 \end{array} \right) = \underbrace{\left( \begin{array}{rrrr} 1 & 0 & 0 & 0\\ 1 & 0 & 0 & 0\\ 0 & 1 & 0 & 0 \\ 0 & 1 & 0 & 0 \\ 0 & 0 & 1 & 0 \\ 0 & 0 & 1 & 0 \\ 0 & 0 & 0 & 1 \\ 0 & 0 & 0 & 1 \end{array} \right)}_{\text{Design Matrix}, \mathbf{X}} \left( \begin{array}{c} \alpha_1 \\ \alpha_2 \\ \alpha_3 \\ \alpha_4 \end{array} \right) + \left( \begin{array}{r} \varepsilon_1 \\ \varepsilon_2 \\ \varepsilon_3\\ \varepsilon_4 \\ \varepsilon_5\\ \varepsilon_6\\ \varepsilon_7\\ \varepsilon_8 \end{array} \right)$

```{r}
x1=iris$Petal.Width
x2=iris$Sepal.Width
y=iris$Sepal.Length
b0=4
b1=0.5
b2=0
learning=0.001
for(i in 1:1000000){
  y_predicted=b0+b1*x1+b2*x2
  b0_gradient=-2/length(x1)*sum((y-y_predicted))
  b1_gradient=-2/length(x1)*sum((y-y_predicted)*x1)
  b2_gradient=-2/length(x2)*sum((y-y_predicted)*x2)
  b0=b0-b0_gradient*learning
  b1=b1-b1_gradient*learning
  b2=b2-b2_gradient*learning
}
c(b0,b1,b2)
lm(iris$Sepal.Length~iris$Petal.Width+iris$Sepal.Width)
```

